x64 crefine: update proofs for explicit fpu changes
Signed-off-by: Corey Lewis <corey.lewis@proofcraft.systems>

proof/crefine/X64/IsolatedThreadAction.thy
@@ -72,13 +72,11 @@ lemma UserContextGet[simp]:
 lemma put_tcb_state_regs_twice[simp]:
   "put_tcb_state_regs tsr (put_tcb_state_regs tsr' tcb)
     = put_tcb_state_regs tsr tcb"
-  apply (simp add: put_tcb_state_regs_def put_tcb_state_regs_tcb_def
-                   makeObject_tcb newArchTCB_def atcbContextSet_def
+  apply (simp add: put_tcb_state_regs_defs makeObject_tcb newArchTCB_def
             split: tcb_state_regs.split option.split
                    Structures_H.kernel_object.split)
-  apply (intro all_tcbI impI allI)
-   using atcbContextSet_def atcbContext_set_set
-   apply fastforce+
+  using atcbContextSet_def atcbContext_set_set
+  apply (intro all_tcbI impI allI conjI; simp)
   done
 
 lemma partial_overwrite_twice[simp]:
@@ -172,14 +170,14 @@ context begin interpretation Arch . (*FIXME: arch-split*)
 lemma get_tcb_state_regs_ko_at':
   "ko_at' ko p s \<Longrightarrow> get_tcb_state_regs (ksPSpace s p)
        = TCBStateRegs (tcbState ko) ((user_regs o atcbContextGet o tcbArch) ko)"
-  by (clarsimp simp: obj_at'_def projectKOs get_tcb_state_regs_def)
+  by (clarsimp simp: obj_at'_def projectKOs get_tcb_state_regs_defs)
 
 lemma put_tcb_state_regs_ko_at':
   "ko_at' ko p s \<Longrightarrow> put_tcb_state_regs tsr (ksPSpace s p)
        = Some (KOTCB (ko \<lparr> tcbState := tsrState tsr
-                         , tcbArch := atcbContextSet (UserContext (user_fpu_state (atcbContext (tcbArch ko))) (tsrContext tsr)) (tcbArch ko)\<rparr>))"
-  by (clarsimp simp: obj_at'_def projectKOs put_tcb_state_regs_def
-                     put_tcb_state_regs_tcb_def
+                         , tcbArch := atcbContextSet (UserContext (user_fpu_state (atcbContext (tcbArch ko)))
+                                                                  (tsrContext tsr)) (tcbArch ko)\<rparr>))"
+  by (clarsimp simp: obj_at'_def projectKOs put_tcb_state_regs_defs
               split: tcb_state_regs.split)
 
 lemma partial_overwrite_get_tcb_state_regs:
@@ -190,7 +188,7 @@ lemma partial_overwrite_get_tcb_state_regs:
                       split: if_split)
   apply clarsimp
   apply (drule_tac x=xa in spec)
-  apply (clarsimp simp: obj_at'_def put_tcb_state_regs_defs get_tcb_state_regs_defs)
+  apply (clarsimp simp: obj_at'_def projectKOs put_tcb_state_regs_defs get_tcb_state_regs_defs)
   apply (case_tac obj, simp)
   done
 
@@ -279,7 +277,7 @@ lemma map_to_ctes_partial_overwrite:
   apply (case_tac "x \<in> range idx")
    apply (clarsimp simp: put_tcb_state_regs_def)
    apply (drule_tac x=xa in spec)
-   apply (clarsimp simp: obj_at'_def objBits_simps'
+   apply (clarsimp simp: obj_at'_def projectKOs objBits_simps'
                    cong: if_cong)
    apply (simp add: put_tcb_state_regs_tcb_def objBits_simps'
               cong: if_cong option.case_cong)
@@ -290,7 +288,7 @@ lemma map_to_ctes_partial_overwrite:
   apply (case_tac "x && ~~ mask (objBitsKO (KOTCB undefined)) \<in> range idx")
    apply (clarsimp simp: put_tcb_state_regs_def)
    apply (drule_tac x=xa in spec)
-   apply (clarsimp simp: obj_at'_def objBits_simps'
+   apply (clarsimp simp: obj_at'_def projectKOs objBits_simps'
                    cong: if_cong)
    apply (simp add: put_tcb_state_regs_tcb_def objBits_simps'
               cong: if_cong option.case_cong)
@@ -535,7 +533,7 @@ lemma thread_actions_isolatable_bind:
   apply (simp add: obj_at_partial_overwrite_If)
   done
 
-lemma thread_actions_isolatable_return:
+lemma thread_actions_isolatable_return[simp]:
   "thread_actions_isolatable idx (return v)"
   apply (clarsimp simp: thread_actions_isolatable_def
                         monadic_rewrite_def liftM_def
@@ -546,19 +544,22 @@ lemma thread_actions_isolatable_return:
                    ksPSpace_update_partial_id)
   done
 
-lemma thread_actions_isolatable_fail:
+lemma thread_actions_isolatable_fail[simp]:
   "thread_actions_isolatable idx fail"
   by (simp add: thread_actions_isolatable_def
                 isolate_thread_actions_def select_f_asserts
                 liftM_def bind_assoc getSchedulerAction_def
                 monadic_rewrite_def exec_gets)
 
-lemma thread_actions_isolatable_returns:
+lemma thread_actions_isolatable_assert[simp]:
+  "thread_actions_isolatable idx (assert P)"
+  by (auto simp: assert_def)
+
+lemma thread_actions_isolatable_returns[simp]:
   "thread_actions_isolatable idx (return v)"
   "thread_actions_isolatable idx (returnOk v)"
   "thread_actions_isolatable idx (throwError v)"
-  by (simp add: returnOk_def throwError_def
-                thread_actions_isolatable_return)+
+  by (simp add: returnOk_def throwError_def)+
 
 lemma thread_actions_isolatable_bindE:
   "\<lbrakk> thread_actions_isolatable idx f; \<And>x. thread_actions_isolatable idx (g x);
@@ -944,7 +945,7 @@ lemma oblivious_switchToThread_schact:
                    tcbQueueRemove_def ksReadyQueues_asrt_def)
   by (safe intro!: oblivious_bind
               | simp_all add: ready_qs_runnable_def idleThreadNotQueued_def
-                              oblivious_setVMRoot_schact)+
+                              oblivious_setVMRoot_schact oblivious_lazyFpuRestore_schact)+
 
 (* FIXME move *)
 lemma empty_fail_getCurThread[intro!, wp, simp]:
@@ -1145,13 +1146,13 @@ lemma setCTE_isolatable:
     apply (rule ext)
     apply (clarsimp simp: partial_overwrite_get_tcb_state_regs
                    split: if_split)
-    apply (clarsimp simp: get_tcb_state_regs_defs put_tcb_state_regs_defs
+    apply (clarsimp simp: projectKOs get_tcb_state_regs_defs put_tcb_state_regs_defs
                           partial_overwrite_def
                    split: tcb_state_regs.split)
     apply (case_tac obj, simp add: projectKO_opt_tcb)
     apply (simp add: tcb_cte_cases_def split: if_split_asm)
    apply (drule_tac x=x in spec)
-   apply (clarsimp simp: obj_at'_def objBits_simps subtract_mask(2) [symmetric])
+   apply (clarsimp simp: obj_at'_def projectKOs objBits_simps subtract_mask(2) [symmetric])
    apply (erule notE[rotated], erule (3) tcb_ctes_clear[rotated])
   apply (simp add: select_f_returns select_f_asserts split: if_split)
   apply (intro conjI impI)
@@ -1227,7 +1228,7 @@ lemma isolate_thread_actions_threadSet_tcbState:
                 intro!: kernel_state.fold_congs[OF refl refl])
   apply (simp add: partial_overwrite_fun_upd
                    partial_overwrite_get_tcb_state_regs)
-  apply (clarsimp simp: put_tcb_state_regs_defs get_tcb_state_regs_defs
+  apply (clarsimp simp: put_tcb_state_regs_defs get_tcb_state_regs_defs projectKOs
                  elim!: obj_atE')
   apply (case_tac ko)
   apply (simp add: projectKO_opt_tcb)
@@ -1278,23 +1279,177 @@ lemma threadGet_isolatable:
   apply (clarsimp simp: exec_gets exec_modify o_def
                         ksPSpace_update_partial_id in_monad)
   apply (erule obj_atE')
-  apply (clarsimp simp: projectKOs
-                        partial_overwrite_def put_tcb_state_regs_def
+  apply (clarsimp simp: projectKOs partial_overwrite_def put_tcb_state_regs_def
                   cong: if_cong)
   apply (simp add: projectKO_opt_tcb v split: if_split)
   done
 
- lemma switchToThread_isolatable:
-  "thread_actions_isolatable idx (Arch.switchToThread t)"
-  apply (simp add: switchToThread_def
-                   storeWordUser_def stateAssert_def2)
+lemma typ_at_partial_overwrite_id2:
+  "\<lbrakk> \<forall>x. tcb_at' (idx x) s \<rbrakk>
+   \<Longrightarrow> typ_at' P p (ksPSpace_update (partial_overwrite idx f) s) = typ_at' P p s"
+  apply (frule dom_partial_overwrite[where tsrs=f])
+  apply (clarsimp simp: typ_at'_def ko_wp_at'_def obj_at'_def ps_clear_def partial_overwrite_def projectKOs)
+  apply (drule_tac x=x in spec)
+  apply (clarsimp simp: put_tcb_state_regs_def objBits_simps)
+  done
+
+lemma tcb_at_partial_overwrite:
+  "\<forall>x. tcb_at' (idx x) s \<Longrightarrow>
+   tcb_at' p (ksPSpace_update (partial_overwrite idx f) s) = tcb_at' p s"
+  by (simp add: tcb_at_typ_at' typ_at_partial_overwrite_id2)
+
+
+definition asUserFPU :: "machine_word \<Rightarrow> (fpu_state \<Rightarrow> ('a \<times> fpu_state)) \<Rightarrow> 'a kernel" where
+  "asUserFPU tptr f \<equiv> do
+        fpu \<leftarrow> threadGet (user_fpu_state \<circ> atcbContextGet o tcbArch) tptr;
+        threadSet (\<lambda>tcb. tcb \<lparr> tcbArch := atcbContextSet (UserContext (snd (f fpu)) (user_regs (atcbContext (tcbArch tcb))))
+                                           (tcbArch tcb)\<rparr>) tptr;
+        return (fst (f fpu))
+   od"
+
+lemma asUser_asUserFPU_set:
+  "asUser t (setFPUState fc) = asUserFPU t (\<lambda>_. ((), fc))"
+  unfolding asUser_def asUserFPU_def setFPUState_def
+  apply (clarsimp simp: select_f_returns threadGet_stateAssert_gets bind_assoc exec_gets comp_def
+                intro!: ext bind_apply_cong[where f="stateAssert P L" for P L, OF refl]
+                 dest!: fst_stateAssertD)
+  apply (clarsimp simp: threadSet_det simpler_modify_def)
+  apply (rule kernel_state.unfold_congs; simp?)
+  apply (rule ext)
+  apply (clarsimp simp: obj_at'_def atcbContextSet_def thread_fetch_def atcbContextGet_def projectKOs)
+  done
+
+lemma asUser_asUserFPU_get:
+  "asUser t getFPUState = asUserFPU t (\<lambda>fc. (fc, fc))"
+  unfolding asUser_def asUserFPU_def getFPUState_def
+  apply (subst threadSet_stateAssert_modify)+
+  apply (clarsimp simp: select_f_returns threadGet_stateAssert_gets bind_assoc exec_gets comp_def
+                intro!: ext bind_apply_cong[where f="stateAssert P L" for P L, OF refl]
+                 dest!: fst_stateAssertD)
+  apply (clarsimp simp: simpler_modify_def return_def bind_def)
+  apply (clarsimp simp: obj_at'_def atcbContextSet_def thread_fetch_def atcbContextGet_def
+                        thread_replace_def projectKOs)
+  done
+
+lemma put_tcb_state_regs_tcb_twice[simp]:
+  "put_tcb_state_regs_tcb tsr (put_tcb_state_regs_tcb tsr' tcb) = put_tcb_state_regs_tcb tsr tcb"
+  apply (cases tcb)
+  apply (simp add: put_tcb_state_regs_tcb_def split: tcb_state_regs.split)
+  apply (fastforce simp: atcbContextSet_def)
+  done
+
+lemma put_tcb_state_regs_tcb_unchanged:
+  "get_tcb_state_regs_tcb tcb = tsr \<Longrightarrow> put_tcb_state_regs_tcb tsr tcb = tcb"
+  apply (cases tcb)
+  apply (clarsimp simp: put_tcb_state_regs_tcb_def get_tcb_state_regs_tcb_def)
+  done
+
+lemma threadSet_isolatable:
+  assumes v: "\<And>tcb. get_tcb_state_regs_tcb (f tcb) = get_tcb_state_regs_tcb tcb"
+  assumes y: "\<And>tsr tcb. f (put_tcb_state_regs_tcb tsr tcb) = put_tcb_state_regs_tcb tsr (f tcb)"
+  shows "thread_actions_isolatable idx (threadSet f t)"
+  apply (clarsimp simp: threadSet_def)
+  apply (subst setObject_assert_modify;
+         simp add: objBits_2n objBits_simps tcbBlockSizeBits_def projectKOs)+
+  apply (clarsimp simp: thread_actions_isolatable_def isolate_thread_actions_def split_def
+                        getObject_get_assert
+                        setObject_assert_modify objBits_2n objBits_simps tcbBlockSizeBits_def liftM_def
+                        state_assert_def
+                        bind_select_f_bind[symmetric]
+                        select_f_returns select_f_asserts bind_assoc)
+  apply (clarsimp simp: monadic_rewrite_def exec_gets
+                        getSchedulerAction_def)
+  apply (simp add: obj_at_partial_overwrite_If)
+  apply (rule bind_apply_cong[OF refl])
+  apply (clarsimp simp: exec_gets exec_get simpler_modify_def o_def
+                        ksPSpace_update_partial_id in_monad)
+  apply (erule obj_atE')
+  apply (rule kernel_state.unfold_congs; simp?)
+  apply (rule ext)
+  apply (clarsimp simp: projectKOs)
+  apply (intro impI conjI)
+   apply (clarsimp simp: partial_overwrite_def put_tcb_state_regs_def get_tcb_state_regs_def
+                         y put_tcb_state_regs_tcb_unchanged v)
+  apply (clarsimp simp: partial_overwrite_def put_tcb_state_regs_def get_tcb_state_regs_def)
+  apply (drule_tac x=xa in spec)
+  apply (clarsimp simp: obj_at'_def put_tcb_state_regs_tcb_unchanged projectKOs)
+  done
+
+lemma atcbContext_update_twice[simp]:
+  "atcbContext_update f (atcbContext_update f' v) = atcbContext_update (f \<circ> f') v"
+  by (cases v; clarsimp)
+
+lemma tcbArch_update_twice[simp]:
+  "tcbArch_update f (tcbArch_update f' v) = tcbArch_update (f \<circ> f') v"
+  by (cases v; clarsimp)
+
+lemma asUserFPU_isolatable:
+  "thread_actions_isolatable idx (asUserFPU t f)"
+  apply (simp add: asUserFPU_def)
   apply (intro thread_actions_isolatable_bind[OF _ _ hoare_weaken_pre]
-               gets_isolatable setVMRoot_isolatable
+               thread_actions_isolatable_returns
+               threadGet_isolatable threadSet_isolatable)
+        apply (wpsimp simp: put_tcb_state_regs_tcb_def get_tcb_state_regs_tcb_def atcbContextGet_def atcbContextSet_def
+                     split: tcb_state_regs.split)+
+      apply (case_tac tcb)
+      apply clarsimp
+     apply wpsimp+
+  done
+
+lemma saveFpuState_isolatable:
+  "thread_actions_isolatable idx (saveFpuState t)"
+  apply (simp add: saveFpuState_def asUser_asUserFPU_set)
+  apply (intro thread_actions_isolatable_bind[OF _ _ hoare_weaken_pre]
+               doMachineOp_isolatable asUserFPU_isolatable
+         | wpsimp)+
+  done
+
+lemma asUserFPU_typ_at'[wp]:
+  "\<lbrace>\<lambda>s. P (typ_at' T p s)\<rbrace> asUserFPU t' f \<lbrace>\<lambda>rv s. P (typ_at' T p s)\<rbrace>"
+  by (simp add: asUserFPU_def bind_assoc split_def, wp select_f_inv)
+
+lemmas asUserFPU_typ_ats[wp] = typ_at_lifts [OF asUserFPU_typ_at']
+
+lemma loadFpuState_isolatable:
+  "thread_actions_isolatable idx (loadFpuState t)"
+  apply (simp add: loadFpuState_def asUser_asUserFPU_get)
+  apply (intro thread_actions_isolatable_bind[OF _ _ hoare_weaken_pre]
+               doMachineOp_isolatable asUserFPU_isolatable
+         | wpsimp)+
+  done
+
+lemma switchLocalFpuOwner_isolatable:
+  "thread_actions_isolatable idx (switchLocalFpuOwner t)"
+  apply (simp add: switchLocalFpuOwner_def stateAssert_def2 fpuOwner_asrt_def case_option_If2
+              split del: if_split)
+  apply (intro thread_actions_isolatable_bind[OF _ _ hoare_weaken_pre]
+               gets_isolatable
                thread_actions_isolatable_if
                doMachineOp_isolatable
+               saveFpuState_isolatable loadFpuState_isolatable modifyArchState_isolatable)
+        apply (wpsimp simp: none_top_def tcb_at_partial_overwrite
+                     split: option.split)+
+  done
+
+lemma lazyFpuRestore_isolatable:
+  "thread_actions_isolatable idx (lazyFpuRestore t)"
+  apply (simp add: lazyFpuRestore_def)
+  apply (intro thread_actions_isolatable_bind[OF _ _ hoare_weaken_pre]
+               gets_isolatable thread_actions_isolatable_if doMachineOp_isolatable
+               threadGet_isolatable [OF all_tcbI] switchLocalFpuOwner_isolatable)
+        apply (wpsimp simp: put_tcb_state_regs_tcb_def
+                     split: tcb_state_regs.split)+
+  done
+
+lemma switchToThread_isolatable:
+  "thread_actions_isolatable idx (Arch.switchToThread t)"
+  apply (simp add: switchToThread_def)
+  apply (intro thread_actions_isolatable_bind[OF _ _ hoare_weaken_pre]
+               setVMRoot_isolatable
+               doMachineOp_isolatable
                threadGet_isolatable [OF all_tcbI]
-               thread_actions_isolatable_returns
-               thread_actions_isolatable_fail)
+               lazyFpuRestore_isolatable)
+   apply wpsimp+
   done
 
 lemma tcbQueued_put_tcb_state_regs_tcb:
@@ -1405,7 +1560,7 @@ lemma set_register_isolate:
                         partial_overwrite_fun_upd
                         partial_overwrite_get_tcb_state_regs)
   apply (drule_tac x=y in spec)
-  apply (clarsimp simp: obj_at'_def objBits_simps
+  apply (clarsimp simp: obj_at'_def projectKOs objBits_simps
                   cong: if_cong)
   apply (case_tac obj)
   apply (simp add: projectKO_opt_tcb put_tcb_state_regs_defs
@@ -1437,7 +1592,7 @@ lemma copy_register_isolate:
                         partial_overwrite_fun_upd
                         partial_overwrite_get_tcb_state_regs)
   apply (frule_tac x=x in spec, drule_tac x=y in spec)
-  apply (clarsimp simp: obj_at'_def objBits_simps
+  apply (clarsimp simp: obj_at'_def projectKOs objBits_simps
                   cong: if_cong)
   apply (case_tac obj, case_tac obja)
   apply (simp add: projectKO_opt_tcb put_tcb_state_regs_defs
