proof/crefine/X64/Machine_C.thy
@@ -37,23 +37,6 @@ assumes ioapicMapPinToVector_ccorres:
      (doMachineOp (ioapicMapPinToVector ioapic pin level polarity vector))
      (Call ioapic_map_pin_to_vector_'proc)"
 
-(* FIXME: x64: Currently don't verify FPU lazy state switching (VER-951) *)
-assumes nativeThreadUsingFPU_ccorres:
-  "ccorres (\<lambda>rv rv'. rv' = from_bool rv) ret__unsigned_long_'
-     (tcb_at' thread)
-     (UNIV \<inter> \<lbrace>\<acute>thread = tcb_ptr_to_ctcb_ptr thread\<rbrace>)
-     []
-     (doMachineOp (nativeThreadUsingFPU thread))
-     (Call nativeThreadUsingFPU_'proc)"
-
-assumes switchFpuOwner_ccorres:
-  "ccorres dc xfdc \<top>
-     (UNIV \<inter> \<lbrace>\<acute>new_owner = Ptr new_owner\<rbrace>
-           \<inter> \<lbrace>\<acute>cpu = cpu\<rbrace>)
-     []
-     (doMachineOp (switchFpuOwner new_owner cpu))
-     (Call switchFpuOwner_'proc)"
-
 (* FIXME x64: double-check this, assumption is ccorres holds regardless of in_kernel *)
 (* FIXME x64: accessor function relation was complicated on ARM, testing if you don't
               need it to be that way *)
